src/llvm-mem/Intptr.v
@@ -1,0 +1,69 @@
+From Coq Require Import
+  ZArith.
+
+From Vellvm Require Import
+  Semantics.VellvmIntegers
+  Utils.Error
+  DynamicTypes.
+
+Module Type INTPTR.
+  Parameter intptr : Set.
+  Parameter zero : intptr.
+
+  Parameter VMemInt_intptr : VMemInt intptr.
+
+  Parameter eq_dec : forall (a b : intptr), {a = b} + {a <> b}.
+  Parameter eqb : forall (a b : intptr), bool.
+
+  Parameter to_Z : forall (a : intptr), Z.
+  Parameter to_unsigned : forall (a : intptr), Z.
+  Parameter from_Z : Z -> OOM intptr.
+
+  Parameter from_Z_to_Z :
+    forall (z : Z) (i : intptr),
+      from_Z z = NoOom i ->
+      to_Z i = z.
+
+  Parameter from_Z_injective :
+    forall (z1 z2 : Z) (i : intptr),
+      from_Z z1 = NoOom i ->
+      from_Z z2 = NoOom i ->
+      z1 = z2.
+
+  Parameter to_Z_from_Z :
+    forall (i : intptr),
+      from_Z (to_Z i) = NoOom i.
+
+  Parameter from_Z_0 :
+    from_Z 0 = NoOom zero.
+
+  Parameter to_Z_0 :
+    to_Z zero = 0%Z.
+
+  Parameter to_Z_inj :
+    forall x y,
+      to_Z x = to_Z y ->
+      x = y.
+
+  Parameter VMemInt_intptr_dtyp :
+    @mdtyp_of_int intptr VMemInt_intptr = DTYPE_IPTR.
+
+  Parameter VMemInt_intptr_mrepr_from_Z :
+    forall x,
+      @mrepr intptr VMemInt_intptr x = from_Z x.
+
+  Parameter to_Z_to_unsigned :
+    forall x,
+      to_Z x = to_unsigned x.
+End INTPTR.
+
+Module Type INTPTR_BIG (IP : INTPTR).
+  Import IP.
+
+  Parameter from_Z_safe :
+    forall z,
+      match from_Z z with
+      | NoOom _ => True
+      | Oom _ => False
+      end.
+End INTPTR_BIG.
