src/mem/Addresses/MemoryAddress.v
@@ -1,0 +1,158 @@
+(* -------------------------------------------------------------------------- *
+ *                     Vellvm - the Verified LLVM project                     *
+ *                                                                            *
+ *     Copyright (c) 2017 Steve Zdancewic <stevez@cis.upenn.edu>              *
+ *                                                                            *
+ *   This file is distributed under the terms of the GNU General Public       *
+ *   License as published by the Free Software Foundation, either version     *
+ *   3 of the License, or (at your option) any later version.                 *
+ ---------------------------------------------------------------------------- *)
+
+(* begin hide *)
+Require Import String.
+Require Import OrderedType OrderedTypeEx.
+Require Import ZArith.
+Require Import Coqlib.
+
+From Vellvm Require Import
+     Utils.Error.
+
+From ExtLib Require Import
+  Structures.Monads.
+
+From Coq Require Import
+  Structures.Equalities.
+
+From Mem Require Import
+  Addresses.Provenance.
+
+Import MonadNotation.
+Open Scope monad_scope.
+(* end hide *)
+
+(*** Abstract address modules *)
+Module ADDRESS_TYPE_NOTATION (Import T:Typ).
+  Notation addr := t.
+End ADDRESS_TYPE_NOTATION.
+
+(** The core abstract address type, which essentially just has
+    decidable equality.
+ *)
+Module Type CORE_ADDRESS := DecidableType <+ ADDRESS_TYPE_NOTATION.
+
+(*** Address functors *)
+
+(** Addresses which have null pointers *)
+Module Type HAS_NULL (Import Addr:CORE_ADDRESS).
+  Parameter null : addr.
+End HAS_NULL.
+
+(** Address types which can be converted to integers *)
+Module Type HAS_PTOI (Import Addr:CORE_ADDRESS).
+  Parameter ptr_to_int : addr -> Z.
+End HAS_PTOI.
+
+Module Type HAS_POINTER_ARITHMETIC (Import Addr:CORE_ADDRESS).
+  (** Pointer addition. May error if the result cannot be represented
+      as a pointer, e.g., if it would be out of bounds.
+   *)
+  Parameter ptr_add : addr -> Z -> err addr.
+End HAS_POINTER_ARITHMETIC.
+
+Module Type PTOI_ARITH_EXTRAS (Import Addr:CORE_ADDRESS) (Import PTOI : HAS_PTOI Addr) (Import HPA : HAS_POINTER_ARITHMETIC Addr).
+  Parameter ptr_to_int_ptr_add :
+    forall (ptr ptr' : addr) (x : Z),
+      ptr_add ptr x = inr ptr' ->
+      ptr_to_int ptr' = ptr_to_int ptr + x.
+End PTOI_ARITH_EXTRAS.
+
+(* TODO: Should this be moved to a utility file? *)
+(** Types with additional metadata associated with them *)
+Module Type HAS_METADATA (METADATA : Typ) (Import T:Typ).
+  Parameter extract_metadata : t -> METADATA.t.
+End HAS_METADATA.
+
+(** Address types which support casts from integers
+
+    METADATA is a type representing any extra metadata that might be
+    needed when constructing a pointer from an integer type. Usually
+    this metadata is something like a provenance.
+ *)
+Module Type HAS_ITOP (METADATA : Typ) (Import Addr:CORE_ADDRESS) (Import HMD : HAS_METADATA METADATA Addr).
+  (** Convert an integer to a pointer.
+
+      Parameters:
+      - The integer to convert to a pointer value.
+      - Metadata associated with the pointer (often this is a provenance).
+
+      Return value:
+      The resulting address. May OOM if the integer value doesn't fit
+      in the address space.
+   *)
+  Parameter int_to_ptr : Z -> METADATA.t -> OOM addr.
+  Parameter int_to_ptr_metadata :
+    forall (x : Z) (p : METADATA.t) (a : addr),
+      int_to_ptr x p = ret a ->
+      extract_metadata a = p.
+End HAS_ITOP.
+
+(** Addresses that integers can safely be converted to (infinite
+    address space)
+ *)
+Module Type ITOP_BIG (METADATA : Typ) (Import Addr:CORE_ADDRESS) (Import HMD : HAS_METADATA METADATA Addr) (Import ITOP : HAS_ITOP METADATA Addr HMD).
+  Parameter int_to_ptr_safe :
+    forall z pr,
+      match int_to_ptr z pr with
+      | NoOom _ => True
+      | Oom _ => False
+      end.
+End ITOP_BIG.
+
+(** Extra properties for addresses that support both ptoi and itop casts *)
+Module Type PTOI_ITOP_EXTRA (METADATA : Typ) (Import Addr:CORE_ADDRESS) (Import HMD : HAS_METADATA METADATA Addr) (Import ITOP : HAS_ITOP METADATA Addr HMD) (Import PTOI : HAS_PTOI Addr).
+  Parameter int_to_ptr_ptr_to_int :
+    forall (a : addr) (p : METADATA.t),
+      extract_metadata a = p ->
+      int_to_ptr (ptr_to_int a) p = ret a.
+
+  Parameter int_to_ptr_ptr_to_int_exists :
+    forall (a : addr) (p : METADATA.t),
+    exists a',
+      int_to_ptr (ptr_to_int a) p = ret a' /\
+        ptr_to_int a' = ptr_to_int a /\
+        extract_metadata a' = p.
+
+  Parameter ptr_to_int_int_to_ptr :
+    forall (x : Z) (p : METADATA.t) (a : addr),
+      int_to_ptr x p = ret a ->
+      ptr_to_int a = x.
+End PTOI_ITOP_EXTRA.
+
+(** Address types with an associated provenance *)
+Module Type HAS_PROVENANCE (Import PS : PROV_SET) (Import Addr:CORE_ADDRESS).
+  (** Access the provenance for an address *)
+  Parameter address_provenance : addr -> ProvSet.
+End HAS_PROVENANCE.
+
+Module HAS_PROVENANCE_TO_HAS_METADATA (Import PS : PROV_SET) (Import Addr:CORE_ADDRESS) (Import HP : HAS_PROVENANCE PS Addr) <: HAS_METADATA PS Addr.
+  Definition extract_metadata := address_provenance.
+End HAS_PROVENANCE_TO_HAS_METADATA.
+
+(*** Address module types *)
+(** Addresses that can be null *)
+Module Type NULLABLE_ADDRESSES := CORE_ADDRESS <+ HAS_NULL.
+
+(** Addresses with the batteries included *)
+Module Type ADDRESS :=
+  CORE_ADDRESS <+ HAS_NULL <+ HAS_POINTER_ARITHMETIC <+
+    HAS_PROVENANCE <+ HAS_PROVENANCE_TO_HAS_METADATA <+
+    HAS_PTOI <+ HAS_ITOP <+ PTOI_ITOP_EXTRA <+ PTOI_ARITH_EXTRAS.
+
+(** Infinite addresses with the batteries included *)
+Module Type INFINITE_ADDRESS :=
+  ADDRESS <+ ITOP_BIG.
+
+(* TODO: Move this to a show utility file? *)
+Module Type SHOWABLE (Import T:Typ).
+  Parameter show_t : t -> string.
+End SHOWABLE.
