src/mem/Semantics/Memory/StoreId.v
@@ -1,0 +1,3 @@
+Require Import ZArith.
+
+Definition store_id := N.
